theories/language/weakestpre.v
@@ -1,0 +1,516 @@
+From iris.proofmode Require Import base proofmode classes.
+From iris.base_logic.lib Require Export fancy_updates.
+From melocoton.language Require Export language.
+(* FIXME: If we import iris.bi.weakestpre earlier texan triples do not
+   get pretty-printed correctly. *)
+From iris.bi Require Export weakestpre.
+From iris.prelude Require Import options.
+Import uPred.
+
+Class irisGS_gen 
+  (hlc : has_lc) (val pubstate : Type) 
+  (Λ : language val pubstate) (Σ : gFunctors) := IrisG {
+  iris_invGS :> invGS_gen hlc Σ;
+
+  (** The state interpretation is an invariant that should hold in
+  between each step of reduction. Here [Λstate] is the global state,
+  the first [nat] is the number of steps already performed by the
+  program, [list (observation Λ)] are the remaining observations, and the
+  last [nat] is the number of forked-off threads (not the total number
+  of threads, which is one higher because there is always a main
+  thread). *)
+  state_interp : state Λ → nat → iProp Σ;
+
+  (** When performing pure steps, the state interpretation needs to be
+  adapted for the change in the [ns] parameter.
+
+  Note that we use an empty-mask fancy update here. We could also use
+  a basic update or a bare magic wand, the expressiveness of the
+  framework would be the same. If we removed the modality here, then
+  the client would have to include the modality it needs as part of
+  the definition of [state_interp]. Since adding the modality as part
+  of the definition [state_interp_mono] does not significantly
+  complicate the formalization in Iris, we prefer simplifying the
+  client. *)
+  state_interp_mono σ ns:
+    state_interp σ ns ={∅}=∗ state_interp σ (S ns)
+}.
+Global Opaque iris_invGS.
+Global Arguments IrisG {hlc val pubstate Λ Σ}.
+
+Notation irisGS := (irisGS_gen HasLc).
+(** The predicate we take the fixpoint of in order to define the WP. *)
+(** In the step case, we both provide [S (num_laters_per_step ns)]
+  later credits, as well as an iterated update modality that allows
+  stripping as many laters, where [ns] is the number of steps already taken.
+  We have both as each of these provides distinct advantages:
+  - Later credits do not have to be used right away, but can be kept to
+    eliminate laters at a later point.
+  - The step-taking update composes well in parallel: we can independently
+    compose two clients who want to eliminate their laters for the same
+    physical step, which is not possible with later credits, as they
+    can only be used by exactly one client.
+  - The step-taking update can even be used by clients that opt out of
+    later credits, e.g. because they use [BiFUpdPlainly]. *)
+Definition wp_pre `{!irisGS_gen hlc val pubstate Λ Σ} 
+    (p:mixin_prog Λ.(func))
+    (T: string -d> list val -d> (val -d> iPropO Σ) -n> iPropO Σ)
+    (wp : coPset -d>
+          expr Λ -d>
+          (val -d> iPropO Σ) -d>
+          iPropO Σ) :
+    coPset -d>
+    expr Λ -d>
+    (val -d> iPropO Σ) -d>
+    iPropO Σ := λ E e Φ,
+  (  (∃ v, ⌜e = of_class Λ (ExprVal v)⌝ ∗ (|={E}=> Φ v))
+   ∨ (∃ s vv K, ⌜e = fill K (of_class Λ (ExprCall s vv))⌝ ∗ ⌜p !! s = None⌝ ∗
+        (∀ σ ns, state_interp σ ns ={E}▷=∗ 
+                 (state_interp σ ns ∗ T s vv (λ r, wp E (fill K (of_class Λ (ExprVal r))) Φ))))
+   ∨ (∀ σ1 ns, state_interp σ1 ns ={E,∅}=∗ ⌜reducible p e σ1⌝ ∗
+        ∀ σ2 e', ⌜head_step p e σ1 e' σ2 []⌝ -∗ |={∅}=> ▷ |={∅,E}=> 
+            (state_interp σ2 (S ns) ∗ wp E e' Φ)))%I.
+
+Local Instance wp_pre_contractive `{!irisGS_gen hlc val pubstate Λ Σ}
+     {p:mixin_prog Λ.(func)} T : Contractive (wp_pre p T).
+Proof.
+  rewrite /wp_pre /= => n wp wp' Hwp E e1 Φ. cbn in Hwp.
+  repeat (f_contractive || f_equiv || apply Hwp || intros ?).
+Qed.
+
+Record prog_environ `{!irisGS_gen hlc val pubstate Λ Σ} := {
+  prog : mixin_prog (func Λ);
+  T : string -d> list val -d> (val -d> iPropO Σ) -n> iPropO Σ;
+  T_weak : ∀ s vv Φ Ψ, (∀ r, Φ r -∗ Ψ r) -∗ T s vv Φ -∗ T s vv Ψ
+}.
+
+Local Definition wp_def `{!irisGS_gen hlc val pubstate Λ Σ} : Wp (iProp Σ) (expr Λ) (val) (prog_environ) :=
+  λ p : (prog_environ), fixpoint (wp_pre (p.(prog)) (p.(T))).
+Local Definition wp_aux : seal (@wp_def). Proof. by eexists. Qed.
+Definition wp' := wp_aux.(unseal).
+Global Arguments wp' {hlc val pubstate Λ Σ _}.
+Global Existing Instance wp'.
+Local Lemma wp_unseal `{!irisGS_gen hlc val pubstate Λ Σ} : wp = @wp_def hlc val pubstate Λ Σ _.
+Proof. rewrite -wp_aux.(seal_eq) //. Qed.
+
+Section wp.
+Context `{!irisGS_gen hlc val pubstate Λ Σ}.
+Implicit Types P : iProp Σ.
+Implicit Types Φ : val → iProp Σ.
+Implicit Types v : val.
+Implicit Types e : expr Λ.
+Implicit Types T : string -d> list val -d> (val -d> iPropO Σ) -n> iPropO Σ.
+Implicit Types prog : mixin_prog (func Λ).
+Implicit Types pe : prog_environ.
+
+(* Weakest pre *)
+Lemma wp_unfold pe E e Φ :
+  WP e @ pe; E {{ Φ }} ⊣⊢ wp_pre (pe.(prog)) (pe.(T)) (wp (PROP:=iProp Σ) pe) E e Φ.
+Proof. rewrite wp_unseal. apply (fixpoint_unfold (wp_pre (pe.(prog)) (pe.(T)))). Qed.
+
+Global Instance wp_ne pe E e n :
+  Proper (pointwise_relation _ (dist n) ==> dist n) (wp (PROP:=iProp Σ) pe E e).
+Proof.
+  revert e. induction (lt_wf n) as [n _ IH]=> e Φ Ψ HΦ.
+  rewrite !wp_unfold /wp_pre /=.
+  do 15 f_equiv.
+  1: f_equiv.
+  all: f_contractive.
+  all: f_equiv.
+  all: f_equiv. 
+  1: f_equiv; intros r. 
+  all: apply IH; eauto; intros k; eapply dist_le', HΦ; lia.
+Qed.
+Global Instance wp_proper pe E e :
+  Proper (pointwise_relation _ (≡) ==> (≡)) (wp (PROP:=iProp Σ) pe E e).
+Proof.
+  by intros Φ Φ' ?; apply equiv_dist=>n; apply wp_ne=>v; apply equiv_dist.
+Qed.
+
+Global Instance wp_contractive pe E e n :
+  (∀ v,e <> of_class Λ (ExprVal v)) ->
+  Proper (pointwise_relation _ (dist_later n) ==> dist n) (wp (PROP:=iProp Σ) pe E e).
+Proof.
+  intros Hne Φ Ψ HΦ. rewrite !wp_unfold /wp_pre /=. f_equiv.
+  1: admit. (* TODO: this holds by assumption, if we tie it out of the model? *)
+  do 14 f_equiv.
+  1: f_equiv.
+  all: f_contractive.
+  all: f_equiv.
+  all: f_equiv.
+  1: f_equiv; intros r.
+  all: f_equiv.
+  all: intros v'; apply dist_later_dist, HΦ.
+Admitted.
+
+Lemma wp_value_fupd' pe E Φ v : WP (of_class Λ (ExprVal v)) @ pe; E {{ Φ }} ⊣⊢ |={E}=> Φ v.
+Proof. rewrite wp_unfold /wp_pre. iSplit; first iIntros "[(%x & %Heq & H)|[(%s & %vv & %K & %H1 & _ & H3)|H3]]".
+  - assert (v = x) as ->.
+    1: {assert (to_class (of_class Λ (ExprVal v)) = Some (ExprVal v)) by apply to_of_class.
+        rewrite Heq in H. rewrite to_of_class in H. congruence. }
+    iApply "H".
+  - exfalso. pose proof (fill_val K (of_class Λ (ExprCall s vv))) as Hnv. unfold to_val in Hnv.
+    rewrite to_of_class in Hnv. eapply is_Some_None. apply Hnv.
+    rewrite <- H1. rewrite to_of_class. easy.
+  - admit. (* Can be shown if the state interpretation is unconditionally true for some state *)
+  - iIntros "H". iLeft. iExists v. iSplit; first done. iApply "H".
+Admitted.
+
+
+Definition prog_environ_mono pe1 pe2 : Prop := 
+   prog pe1 = prog pe2
+/\ ∀ (s:string) vv Φ Ψ, (∀ r, Φ r -∗ Ψ r) -∗ T pe1 s vv Φ -∗ T pe2 s vv Ψ.
+
+Lemma wp_strong_mono pe1 pe2 E1 E2 e Φ Ψ :
+  E1 ⊆ E2 → prog_environ_mono pe1 pe2 ->
+  WP e @ pe1; E1 {{ Φ }} -∗ (∀ v, Φ v ={E2}=∗ Ψ v) -∗ WP e @ pe2; E2 {{ Ψ }}.
+Proof.
+  iIntros (HE (Hpe1 & Hpe2)) "H HΦ". iLöb as "IH" forall (e E1 E2 HE Φ Ψ).
+  rewrite !wp_unfold /wp_pre /=.
+  iDestruct "H" as "[(%x & -> & H)|[(%s & %vv & %K & -> & H2 & H3)|H3]]".
+  - iLeft. iExists x. iSplitR; first done. 
+    iApply ("HΦ" with "[> -]"). by iApply (fupd_mask_mono E1 _); first apply HE.
+  - iRight; iLeft. iExists s, vv, K. iSplitR; first done. rewrite Hpe1; iFrame.
+    iIntros "%σ %ns Hσ".
+    iSpecialize ("H3" $! σ ns with "Hσ").
+    iMod (fupd_mask_subseteq E1) as "Hclose"; first done.
+    iMod "H3".
+    iMod "Hclose".
+    do 2 iModIntro.
+    iMod (fupd_mask_subseteq E1) as "Hclose2"; first done.
+    iMod "H3".
+    iMod "Hclose2". iModIntro.
+    iDestruct "H3" as "(Hσ & HT)".
+    iFrame.
+    iApply (Hpe2 s vv with "[HΦ] HT").
+    iIntros "%r H1". iApply ("IH" $! (fill K (of_class Λ (ExprVal r))) E1 E2 HE Φ Ψ with "[H1] HΦ").
+    done.
+  - do 2 iRight. iIntros "%σ1 %ns Hσ".
+    iSpecialize ("H3" $! σ1 ns with "Hσ"). 
+    iMod (fupd_mask_subseteq E1) as "Hclose"; first done.
+    iMod "H3" as "(HH & H3)".
+    iModIntro. rewrite Hpe1. iFrame. iIntros "%σ2 %e' Hstep".
+    iSpecialize ("H3" $! σ2 e' with "Hstep").
+    iMod "H3". iModIntro.
+    iModIntro. iMod "H3" as "(Hσ & HWP)". iMod "Hclose".
+    iModIntro. iFrame. iApply ("IH" $! e' E1 E2 HE Φ Ψ with "HWP HΦ").
+Qed.
+
+Lemma fupd_wp pe E e Φ : (|={E}=> WP e @ pe; E {{ Φ }}) ⊢ WP e @ pe; E {{ Φ }}.
+Proof.
+  rewrite wp_unfold /wp_pre. iIntros "H". (*destruct (to_val e) as [v|] eqn:?.
+  { by iMod "H". }
+  iIntros (σ1 ns κ κs nt) "Hσ1". iMod "H". by iApply "H".
+Qed.
+Lemma wp_fupd s E e Φ : WP e @ s; E {{ v, |={E}=> Φ v }} ⊢ WP e @ s; E {{ Φ }}.
+Proof. iIntros "H". iApply (wp_strong_mono s s E with "H"); auto. Qed.
+
+Lemma wp_atomic s E1 E2 e Φ `{!Atomic (stuckness_to_atomicity s) e} :
+  (|={E1,E2}=> WP e @ s; E2 {{ v, |={E2,E1}=> Φ v }}) ⊢ WP e @ s; E1 {{ Φ }}.
+Proof.
+  iIntros "H". rewrite !wp_unfold /wp_pre.
+  destruct (to_val e) as [v|] eqn:He.
+  { by iDestruct "H" as ">>> $". }
+  iIntros (σ1 ns κ κs nt) "Hσ". iMod "H". iMod ("H" $! σ1 with "Hσ") as "[$ H]".
+  iModIntro. iIntros (e2 σ2 efs Hstep) "Hcred".
+  iApply (step_fupdN_wand with "(H [//] Hcred)").
+  iIntros ">(Hσ & H & Hefs)". destruct s.
+  - rewrite !wp_unfold /wp_pre. destruct (to_val e2) as [v2|] eqn:He2.
+    + iDestruct "H" as ">> $". by iFrame.
+    + iMod ("H" $! _ _ [] with "[$]") as "[H _]". iDestruct "H" as %(? & ? & ? & ? & ?).
+      by edestruct (atomic _ _ _ _ _ Hstep).
+  - destruct (atomic _ _ _ _ _ Hstep) as [v <-%of_to_val].
+    rewrite wp_value_fupd'. iMod "H" as ">H".
+    iModIntro. iFrame "Hσ Hefs". by iApply wp_value_fupd'.
+Qed.
+
+(** This lemma gives us access to the later credits that are generated in each step,
+  assuming that we have instantiated [num_laters_per_step] with a non-trivial (e.g. linear)
+  function.
+  This lemma can be used to provide a "regeneration" mechanism for later credits.
+  [state_interp] will have to be defined in a way that involves the required regneration
+  tokens. TODO: point to an example of how this is used.
+
+  In detail, a client can use this lemma as follows:
+  * the client obtains the state interpretation [state_interp _ ns _ _],
+  * it uses some ghost state wired up to the interpretation to know that
+    [ns = k + m], and update the state interpretation to [state_interp _ m _ _],
+  * _after_ [e] has finally stepped, we get [num_laters_per_step k] later credits
+    that we can use to prove [P] in the postcondition, and we have to update
+    the state interpretation from [state_interp _ (S m) _ _] to
+    [state_interp _ (S ns) _ _] again. *)
+Lemma wp_credit_access s E e Φ P :
+  TCEq (to_val e) None →
+  (∀ m k, num_laters_per_step m + num_laters_per_step k ≤ num_laters_per_step (m + k)) →
+  (∀ σ1 ns κs nt, state_interp σ1 ns κs nt ={E}=∗
+    ∃ k m, state_interp σ1 m κs nt ∗ ⌜ns = (m + k)%nat⌝ ∗
+    (∀ nt σ2 κs, £ (num_laters_per_step k) -∗ state_interp σ2 (S m) κs nt ={E}=∗
+      state_interp σ2 (S ns) κs nt ∗ P)) -∗
+  WP e @ s; E {{ v, P ={E}=∗ Φ v }} -∗
+  WP e @ s; E {{ Φ }}.
+Proof.
+  rewrite !wp_unfold /wp_pre /=. iIntros (-> Htri) "Hupd Hwp".
+  iIntros (σ1 ns κ κs nt) "Hσ1".
+  iMod ("Hupd" with "Hσ1") as (k m) "(Hσ1 & -> & Hpost)".
+  iMod ("Hwp" with "Hσ1") as "[$ Hwp]". iModIntro.
+  iIntros (e2 σ2 efs Hstep) "Hc".
+  iDestruct "Hc" as "[Hone Hc]".
+  iPoseProof (lc_weaken with "Hc") as "Hc"; first apply Htri.
+  iDestruct "Hc" as "[Hm Hk]".
+  iCombine "Hone Hm" as "Hm".
+  iApply (step_fupd_wand with "(Hwp [//] Hm)"). iIntros "Hwp".
+  iApply (step_fupdN_le (num_laters_per_step m)); [ | done | ].
+  { etrans; last apply Htri. lia. }
+  iApply (step_fupdN_wand with "Hwp"). iIntros ">(SI & Hwp & $)".
+  iMod ("Hpost" with "Hk SI") as "[$ HP]". iModIntro.
+  iApply (wp_strong_mono with "Hwp"); [by auto..|].
+  iIntros (v) "HΦ". iApply ("HΦ" with "HP").
+Qed.
+
+(** In this stronger version of [wp_step_fupdN], the masks in the
+   step-taking fancy update are a bit weird and somewhat difficult to
+   use in practice. Hence, we prove it for the sake of completeness,
+   but [wp_step_fupdN] is just a little bit weaker, suffices in
+   practice and is easier to use.
+
+   See the statement of [wp_step_fupdN] below to understand the use of
+   ordinary conjunction here. *)
+Lemma wp_step_fupdN_strong n s E1 E2 e P Φ :
+  TCEq (to_val e) None → E2 ⊆ E1 →
+  (∀ σ ns κs nt, state_interp σ ns κs nt
+       ={E1,∅}=∗ ⌜n ≤ S (num_laters_per_step ns)⌝) ∧
+  ((|={E1,E2}=> |={∅}▷=>^n |={E2,E1}=> P) ∗
+    WP e @ s; E2 {{ v, P ={E1}=∗ Φ v }}) -∗
+  WP e @ s; E1 {{ Φ }}.
+Proof.
+  destruct n as [|n].
+  { iIntros (_ ?) "/= [_ [HP Hwp]]".
+    iApply (wp_strong_mono with "Hwp"); [done..|].
+    iIntros (v) "H". iApply ("H" with "[>HP]"). by do 2 iMod "HP". }
+  rewrite !wp_unfold /wp_pre /=. iIntros (-> ?) "H".
+  iIntros (σ1 ns κ κs nt) "Hσ".
+  destruct (decide (n ≤ num_laters_per_step ns)) as [Hn|Hn]; first last.
+  { iDestruct "H" as "[Hn _]". iMod ("Hn" with "Hσ") as %?. lia. }
+  iDestruct "H" as "[_ [>HP Hwp]]". iMod ("Hwp" with "[$]") as "[$ H]". iMod "HP".
+  iIntros "!>" (e2 σ2 efs Hstep) "Hcred". iMod ("H" $! e2 σ2 efs with "[% //] Hcred") as "H".
+  iIntros "!>!>". iMod "H". iMod "HP". iModIntro.
+  revert n Hn. generalize (num_laters_per_step ns)=>n0 n Hn.
+  iInduction n as [|n] "IH" forall (n0 Hn).
+  - iApply (step_fupdN_wand with "H"). iIntros ">($ & Hwp & $)". iMod "HP".
+    iModIntro. iApply (wp_strong_mono with "Hwp"); [done|set_solver|].
+    iIntros (v) "HΦ". iApply ("HΦ" with "HP").
+  - destruct n0 as [|n0]; [lia|]=>/=. iMod "HP". iMod "H". iIntros "!> !>".
+    iMod "HP". iMod "H". iModIntro. iApply ("IH" with "[] HP H").
+    auto with lia.
+Qed.
+
+Lemma wp_bind K `{!LanguageCtx K} s E e Φ :
+  WP e @ s; E {{ v, WP K (of_val v) @ s; E {{ Φ }} }} ⊢ WP K e @ s; E {{ Φ }}.
+Proof.
+  iIntros "H". iLöb as "IH" forall (E e Φ). rewrite wp_unfold /wp_pre.
+  destruct (to_val e) as [v|] eqn:He.
+  { apply of_to_val in He as <-. by iApply fupd_wp. }
+  rewrite wp_unfold /wp_pre fill_not_val /=; [|done].
+  iIntros (σ1 step κ κs n) "Hσ". iMod ("H" with "[$]") as "[% H]".
+  iModIntro; iSplit.
+  { destruct s; eauto using reducible_fill. }
+  iIntros (e2 σ2 efs Hstep) "Hcred".
+  destruct (fill_step_inv e σ1 κ e2 σ2 efs) as (e2'&->&?); auto.
+  iMod ("H" $! e2' σ2 efs with "[//] Hcred") as "H". iIntros "!>!>".
+  iMod "H". iModIntro. iApply (step_fupdN_wand with "H"). iIntros "H".
+  iMod "H" as "($ & H & $)". iModIntro. by iApply "IH".
+Qed.
+
+Lemma wp_bind_inv K `{!LanguageCtx K} s E e Φ :
+  WP K e @ s; E {{ Φ }} ⊢ WP e @ s; E {{ v, WP K (of_val v) @ s; E {{ Φ }} }}.
+Proof.
+  iIntros "H". iLöb as "IH" forall (E e Φ). rewrite !wp_unfold /wp_pre /=.
+  destruct (to_val e) as [v|] eqn:He.
+  { apply of_to_val in He as <-. by rewrite !wp_unfold /wp_pre. }
+  rewrite fill_not_val //.
+  iIntros (σ1 ns κ κs nt) "Hσ". iMod ("H" with "[$]") as "[% H]".
+  iModIntro; iSplit.
+  { destruct s; eauto using reducible_fill_inv. }
+  iIntros (e2 σ2 efs Hstep) "Hcred".
+  iMod ("H" $! _ _ _ with "[] Hcred") as "H"; first eauto using fill_step.
+  iIntros "!> !>". iMod "H". iModIntro. iApply (step_fupdN_wand with "H").
+  iIntros "H". iMod "H" as "($ & H & $)". iModIntro. by iApply "IH".
+Qed.
+
+(** * Derived rules *)
+Lemma wp_mono s E e Φ Ψ : (∀ v, Φ v ⊢ Ψ v) → WP e @ s; E {{ Φ }} ⊢ WP e @ s; E {{ Ψ }}.
+Proof.
+  iIntros (HΦ) "H"; iApply (wp_strong_mono with "H"); auto.
+  iIntros (v) "?". by iApply HΦ.
+Qed.
+Lemma wp_stuck_mono s1 s2 E e Φ :
+  s1 ⊑ s2 → WP e @ s1; E {{ Φ }} ⊢ WP e @ s2; E {{ Φ }}.
+Proof. iIntros (?) "H". iApply (wp_strong_mono with "H"); auto. Qed.
+Lemma wp_stuck_weaken s E e Φ :
+  WP e @ s; E {{ Φ }} ⊢ WP e @ E ?{{ Φ }}.
+Proof. apply wp_stuck_mono. by destruct s. Qed.
+Lemma wp_mask_mono s E1 E2 e Φ : E1 ⊆ E2 → WP e @ s; E1 {{ Φ }} ⊢ WP e @ s; E2 {{ Φ }}.
+Proof. iIntros (?) "H"; iApply (wp_strong_mono with "H"); auto. Qed.
+Global Instance wp_mono' s E e :
+  Proper (pointwise_relation _ (⊢) ==> (⊢)) (wp (PROP:=iProp Σ) s E e).
+Proof. by intros Φ Φ' ?; apply wp_mono. Qed.
+Global Instance wp_flip_mono' s E e :
+  Proper (pointwise_relation _ (flip (⊢)) ==> (flip (⊢))) (wp (PROP:=iProp Σ) s E e).
+Proof. by intros Φ Φ' ?; apply wp_mono. Qed.
+
+Lemma wp_value_fupd s E Φ e v : IntoVal e v → WP e @ s; E {{ Φ }} ⊣⊢ |={E}=> Φ v.
+Proof. intros <-. by apply wp_value_fupd'. Qed.
+Lemma wp_value' s E Φ v : Φ v ⊢ WP (of_val v) @ s; E {{ Φ }}.
+Proof. rewrite wp_value_fupd'. auto. Qed.
+Lemma wp_value s E Φ e v : IntoVal e v → Φ v ⊢ WP e @ s; E {{ Φ }}.
+Proof. intros <-. apply wp_value'. Qed.
+
+Lemma wp_frame_l s E e Φ R : R ∗ WP e @ s; E {{ Φ }} ⊢ WP e @ s; E {{ v, R ∗ Φ v }}.
+Proof. iIntros "[? H]". iApply (wp_strong_mono with "H"); auto with iFrame. Qed.
+Lemma wp_frame_r s E e Φ R : WP e @ s; E {{ Φ }} ∗ R ⊢ WP e @ s; E {{ v, Φ v ∗ R }}.
+Proof. iIntros "[H ?]". iApply (wp_strong_mono with "H"); auto with iFrame. Qed.
+
+(** This lemma states that if we can prove that [n] laters are used in
+   the current physical step, then one can perform an n-steps fancy
+   update during that physical step. The resources needed to prove the
+   bound on [n] are not used up: they can be reused in the proof of
+   the WP or in the proof of the n-steps fancy update. In order to
+   describe this unusual resource flow, we use ordinary conjunction as
+   a premise. *)
+Lemma wp_step_fupdN n s E1 E2 e P Φ :
+  TCEq (to_val e) None → E2 ⊆ E1 →
+  (∀ σ ns κs nt, state_interp σ ns κs nt
+       ={E1,∅}=∗ ⌜n ≤ S (num_laters_per_step ns)⌝) ∧
+  ((|={E1∖E2,∅}=> |={∅}▷=>^n |={∅,E1∖E2}=> P) ∗
+    WP e @ s; E2 {{ v, P ={E1}=∗ Φ v }}) -∗
+  WP e @ s; E1 {{ Φ }}.
+Proof.
+  iIntros (??) "H". iApply (wp_step_fupdN_strong with "[H]"); [done|].
+  iApply (and_mono_r with "H"). apply sep_mono_l. iIntros "HP".
+  iMod fupd_mask_subseteq_emptyset_difference as "H"; [|iMod "HP"]; [set_solver|].
+  iMod "H" as "_". replace (E1 ∖ (E1 ∖ E2)) with E2; last first.
+  { set_unfold=>x. destruct (decide (x ∈ E2)); naive_solver. }
+  iModIntro. iApply (step_fupdN_wand with "HP"). iIntros "H".
+  iApply fupd_mask_frame; [|iMod "H"; iModIntro]; [set_solver|].
+  by rewrite difference_empty_L (comm_L (∪)) -union_difference_L.
+Qed.
+Lemma wp_step_fupd s E1 E2 e P Φ :
+  TCEq (to_val e) None → E2 ⊆ E1 →
+  (|={E1}[E2]▷=> P) -∗ WP e @ s; E2 {{ v, P ={E1}=∗ Φ v }} -∗ WP e @ s; E1 {{ Φ }}.
+Proof.
+  iIntros (??) "HR H".
+  iApply (wp_step_fupdN_strong 1 _ E1 E2 with "[-]"); [done|..]. iSplit.
+  - iIntros (????) "_". iMod (fupd_mask_subseteq ∅) as "_"; [set_solver+|].
+    auto with lia.
+  - iFrame "H". iMod "HR" as "$". auto.
+Qed.
+
+Lemma wp_frame_step_l s E1 E2 e Φ R :
+  TCEq (to_val e) None → E2 ⊆ E1 →
+  (|={E1}[E2]▷=> R) ∗ WP e @ s; E2 {{ Φ }} ⊢ WP e @ s; E1 {{ v, R ∗ Φ v }}.
+Proof.
+  iIntros (??) "[Hu Hwp]". iApply (wp_step_fupd with "Hu"); try done.
+  iApply (wp_mono with "Hwp"). by iIntros (?) "$$".
+Qed.
+Lemma wp_frame_step_r s E1 E2 e Φ R :
+  TCEq (to_val e) None → E2 ⊆ E1 →
+  WP e @ s; E2 {{ Φ }} ∗ (|={E1}[E2]▷=> R) ⊢ WP e @ s; E1 {{ v, Φ v ∗ R }}.
+Proof.
+  rewrite [(WP _ @ _; _ {{ _ }} ∗ _)%I]comm; setoid_rewrite (comm _ _ R).
+  apply wp_frame_step_l.
+Qed.
+Lemma wp_frame_step_l' s E e Φ R :
+  TCEq (to_val e) None → ▷ R ∗ WP e @ s; E {{ Φ }} ⊢ WP e @ s; E {{ v, R ∗ Φ v }}.
+Proof. iIntros (?) "[??]". iApply (wp_frame_step_l s E E); try iFrame; eauto. Qed.
+Lemma wp_frame_step_r' s E e Φ R :
+  TCEq (to_val e) None → WP e @ s; E {{ Φ }} ∗ ▷ R ⊢ WP e @ s; E {{ v, Φ v ∗ R }}.
+Proof. iIntros (?) "[??]". iApply (wp_frame_step_r s E E); try iFrame; eauto. Qed.
+
+Lemma wp_wand s E e Φ Ψ :
+  WP e @ s; E {{ Φ }} -∗ (∀ v, Φ v -∗ Ψ v) -∗ WP e @ s; E {{ Ψ }}.
+Proof.
+  iIntros "Hwp H". iApply (wp_strong_mono with "Hwp"); auto.
+  iIntros (?) "?". by iApply "H".
+Qed.
+Lemma wp_wand_l s E e Φ Ψ :
+  (∀ v, Φ v -∗ Ψ v) ∗ WP e @ s; E {{ Φ }} ⊢ WP e @ s; E {{ Ψ }}.
+Proof. iIntros "[H Hwp]". iApply (wp_wand with "Hwp H"). Qed.
+Lemma wp_wand_r s E e Φ Ψ :
+  WP e @ s; E {{ Φ }} ∗ (∀ v, Φ v -∗ Ψ v) ⊢ WP e @ s; E {{ Ψ }}.
+Proof. iIntros "[Hwp H]". iApply (wp_wand with "Hwp H"). Qed.
+Lemma wp_frame_wand s E e Φ R :
+  R -∗ WP e @ s; E {{ v, R -∗ Φ v }} -∗ WP e @ s; E {{ Φ }}.
+Proof.
+  iIntros "HR HWP". iApply (wp_wand with "HWP").
+  iIntros (v) "HΦ". by iApply "HΦ".
+Qed.
+End wp.
+
+(** Proofmode class instances *)
+Section proofmode_classes.
+  Context `{!irisGS_gen hlc Λ Σ}.
+  Implicit Types P Q : iProp Σ.
+  Implicit Types Φ : val Λ → iProp Σ.
+  Implicit Types v : val Λ.
+  Implicit Types e : expr Λ.
+
+  Global Instance frame_wp p s E e R Φ Ψ :
+    (∀ v, Frame p R (Φ v) (Ψ v)) →
+    Frame p R (WP e @ s; E {{ Φ }}) (WP e @ s; E {{ Ψ }}) | 2.
+  Proof. rewrite /Frame=> HR. rewrite wp_frame_l. apply wp_mono, HR. Qed.
+
+  Global Instance is_except_0_wp s E e Φ : IsExcept0 (WP e @ s; E {{ Φ }}).
+  Proof. by rewrite /IsExcept0 -{2}fupd_wp -except_0_fupd -fupd_intro. Qed.
+
+  Global Instance elim_modal_bupd_wp p s E e P Φ :
+    ElimModal True p false (|==> P) P (WP e @ s; E {{ Φ }}) (WP e @ s; E {{ Φ }}).
+  Proof.
+    by rewrite /ElimModal intuitionistically_if_elim
+      (bupd_fupd E) fupd_frame_r wand_elim_r fupd_wp.
+  Qed.
+
+  Global Instance elim_modal_fupd_wp p s E e P Φ :
+    ElimModal True p false (|={E}=> P) P (WP e @ s; E {{ Φ }}) (WP e @ s; E {{ Φ }}).
+  Proof.
+    by rewrite /ElimModal intuitionistically_if_elim
+      fupd_frame_r wand_elim_r fupd_wp.
+  Qed.
+
+  Global Instance elim_modal_fupd_wp_atomic p s E1 E2 e P Φ :
+    ElimModal (Atomic (stuckness_to_atomicity s) e) p false
+            (|={E1,E2}=> P) P
+            (WP e @ s; E1 {{ Φ }}) (WP e @ s; E2 {{ v, |={E2,E1}=> Φ v }})%I | 100.
+  Proof.
+    intros ?. by rewrite intuitionistically_if_elim
+      fupd_frame_r wand_elim_r wp_atomic.
+  Qed.
+
+  Global Instance add_modal_fupd_wp s E e P Φ :
+    AddModal (|={E}=> P) P (WP e @ s; E {{ Φ }}).
+  Proof. by rewrite /AddModal fupd_frame_r wand_elim_r fupd_wp. Qed.
+
+  Global Instance elim_acc_wp_atomic {X} E1 E2 α β γ e s Φ :
+    ElimAcc (X:=X) (Atomic (stuckness_to_atomicity s) e)
+            (fupd E1 E2) (fupd E2 E1)
+            α β γ (WP e @ s; E1 {{ Φ }})
+            (λ x, WP e @ s; E2 {{ v, |={E2}=> β x ∗ (γ x -∗? Φ v) }})%I | 100.
+  Proof.
+    iIntros (?) "Hinner >Hacc". iDestruct "Hacc" as (x) "[Hα Hclose]".
+    iApply (wp_wand with "(Hinner Hα)").
+    iIntros (v) ">[Hβ HΦ]". iApply "HΦ". by iApply "Hclose".
+  Qed.
+
+  Global Instance elim_acc_wp_nonatomic {X} E α β γ e s Φ :
+    ElimAcc (X:=X) True (fupd E E) (fupd E E)
+            α β γ (WP e @ s; E {{ Φ }})
+            (λ x, WP e @ s; E {{ v, |={E}=> β x ∗ (γ x -∗? Φ v) }})%I.
+  Proof.
+    iIntros (_) "Hinner >Hacc". iDestruct "Hacc" as (x) "[Hα Hclose]".
+    iApply wp_fupd.
+    iApply (wp_wand with "(Hinner Hα)").
+    iIntros (v) ">[Hβ HΦ]". iApply "HΦ". by iApply "Hclose".
+  Qed.
+End proofmode_classes.
+*)
+Admitted.
+End wp.
